rustfrontend/ElaborateDrop.v
@@ -225,19 +225,25 @@ End ELABORATE.
 
 Local Open Scope error_monad_scope.
 
-Definition init_drop_flag (mayinit: PathsMap.t) (mayuninit: PathsMap.t) (elt: place * ident) : statement :=
-  let (p, flag) := elt in    
-  let id := local_of_place p in
-  match mayinit!id, mayuninit!id with
-  | Some init, Some uninit =>
-      if Paths.mem p init then
-        set_dropflag flag true
-      else
-        if Paths.mem p uninit then
-          set_dropflag flag false
-        else Sskip
-  | _, _ => Sskip
-  end.
+Definition init_drop_flag (mayinit mayuninit universe: PathsMap.t) (elt: place * ident) : statement :=
+  let (p, flag) := elt in
+  if must_owned mayinit mayuninit universe p then
+    set_dropflag flag true
+  else
+    (* how to show that must_owned = false is must_unowed in function
+    entry *)
+    set_dropflag flag false.                 
+  (* let id := local_of_place p in *)
+  (* match mayinit!id, mayuninit!id with *)
+  (* | Some init, Some uninit => *)
+  (*     if Paths.mem p init then *)
+  (*       set_dropflag flag true *)
+  (*     else *)
+  (*       if Paths.mem p uninit then *)
+  (*         set_dropflag flag false *)
+  (*       else Sskip *)
+  (* | _, _ => Sskip *)
+  (* end. *)
 
 (* instance of [get_an] *)
 Definition get_init_info (an: (PMap.t PathsMap.t * PMap.t PathsMap.t * PathsMap.t)) (pc: node) : PathsMap.t * PathsMap.t * PathsMap.t :=
@@ -259,7 +265,7 @@ Definition transf_function (ce: composite_env) (f: function) : Errors.res functi
   let entry_init := mayinit!!entry in
   let entry_uninit := mayuninit!!entry in
   (* init drop flags: if no flags, it would be a Sskip *)
-  let init_stmt := makeseq (map (init_drop_flag entry_init entry_uninit) flags) in
+  let init_stmt := makeseq (map (init_drop_flag entry_init entry_uninit universe) flags) in
   let flag_vars := combine (map snd flags) (repeat type_bool (length flags)) in
   Errors.OK (mkfunction f.(fn_generic_origins)
                         f.(fn_origins_relation)
